Adding KMSKeyring as well as supporting util/extern code.

src/extern/dotnet/KMS.cs
@@ -1,0 +1,110 @@
+using System;
+using System.Collections.Generic;
+using System.IO;
+using System.Linq;
+using System.Text;
+
+using Amazon;
+
+using KMS = Amazon.KeyManagementService;
+using DString = Dafny.Sequence<char>;
+using byteseq = Dafny.Sequence<byte>;
+using EncryptionContext = Dafny.Sequence<_System.Tuple2<Dafny.Sequence<byte>,Dafny.Sequence<byte>>>;
+
+namespace KMSUtils {
+    public partial class __default {
+        public static KMSClient GetClient(DString region) {
+            return new KMSClient(new KMS.AmazonKeyManagementServiceClient(RegionEndpoint.GetBySystemName(region.ToString())));
+        }
+        //TODO: #54
+        public static Dictionary<String, String> EncryptionContextToString(EncryptionContext encContext) {
+            UTF8Encoding utf8 = new UTF8Encoding(false, true);
+            Dictionary<string, string> strDict = encContext.Elements.ToDictionary(
+                    strKey => utf8.GetString((byte[])strKey._0.Elements.Clone()),
+                    strElm => utf8.GetString((byte[])strElm._1.Elements.Clone())
+                    );
+            return strDict;
+        }
+
+        //TODO: #54
+        public static ResponseMetadata ConvertMetaData(Amazon.Runtime.ResponseMetadata rmd) {
+            Dafny.Map<DString, DString> metadata = Dafny.Map<DString, DString>.FromCollection(rmd.Metadata.Select(kvp => new Dafny.Pair<DString, DString>(new DString(kvp.Key.ToCharArray()), new DString(kvp.Value.ToCharArray()))).ToList());
+            DString requestID = new DString(rmd.RequestId.ToCharArray());
+            return new ResponseMetadata(metadata, requestID);
+        }
+    }
+    public partial class KMSClient {
+
+        readonly private KMS.AmazonKeyManagementServiceClient client;
+
+        public KMSClient(KMS.AmazonKeyManagementServiceClient client) {
+            this.client = client;
+        }
+
+        public STL.Result<GenerateDataKeyResponse> GenerateDataKey(GenerateDataKeyRequest request) {
+            try {
+            KMS.Model.GenerateDataKeyRequest kmsRequest = new KMS.Model.GenerateDataKeyRequest()
+            {
+                EncryptionContext = __default.EncryptionContextToString(request.encryptionContext),
+                GrantTokens = request.grantTokens.Elements.Select(element => element.ToString()).ToList(),
+                KeyId = request.keyID.ToString(),
+                NumberOfBytes = request.numberOfBytes
+            };
+            KMS.Model.GenerateDataKeyResponse response = this.client.GenerateDataKey(kmsRequest);
+            return new STL.Result_Success<GenerateDataKeyResponse>(new GenerateDataKeyResponse(
+                    new byteseq(response.CiphertextBlob.GetBuffer()),
+                    response.ContentLength,
+                    (int)response.HttpStatusCode,
+                    new DString(response.KeyId.ToCharArray()),
+                    new byteseq(response.Plaintext.GetBuffer()),
+                    __default.ConvertMetaData(response.ResponseMetadata)
+                    ));
+            } catch {
+                return new STL.Result_Failure<GenerateDataKeyResponse>(new Dafny.Sequence<char>("Exception in KMS.GenerateDataKey()".ToCharArray()));
+            }
+        }
+
+        public STL.Result<EncryptResponse> Encrypt(EncryptRequest request) {
+            try {
+                KMS.Model.EncryptRequest kmsRequest = new KMS.Model.EncryptRequest()
+                {
+                    EncryptionContext = __default.EncryptionContextToString(request.encryptionContext),
+                    GrantTokens = request.grantTokens.Elements.Select(element => element.ToString()).ToList(),
+                    KeyId = request.keyID.ToString(),
+                    Plaintext = new MemoryStream((byte[])request.plaintext.Elements.Clone())
+                };
+                KMS.Model.EncryptResponse response = this.client.Encrypt(kmsRequest);
+                return new STL.Result_Success<EncryptResponse>(new EncryptResponse(
+                            new byteseq(response.CiphertextBlob.GetBuffer()),
+                            response.ContentLength,
+                            (int)response.HttpStatusCode,
+                            new DString(response.KeyId.ToCharArray()),
+                            __default.ConvertMetaData(response.ResponseMetadata)
+                            ));
+            } catch {
+                return new STL.Result_Failure<EncryptResponse>(new Dafny.Sequence<char>("Exception in KMS.Encrypt()".ToCharArray()));
+            }
+        }
+
+        public STL.Result<DecryptResponse> Decrypt(DecryptRequest request) {
+            try {
+                KMS.Model.DecryptRequest kmsRequest = new KMS.Model.DecryptRequest()
+                {
+                    CiphertextBlob = new MemoryStream((byte[])request.ciphertextBlob.Elements.Clone()),
+                    EncryptionContext = __default.EncryptionContextToString(request.encryptionContext),
+                    GrantTokens = request.grantTokens.Elements.Select(element => element.ToString()).ToList(),
+                };
+                KMS.Model.DecryptResponse response = this.client.Decrypt(kmsRequest);
+                return new STL.Result_Success<DecryptResponse>(new DecryptResponse(
+                            response.ContentLength,
+                            (int)response.HttpStatusCode,
+                            new DString(response.KeyId.ToCharArray()),
+                            new byteseq(response.Plaintext.GetBuffer()),
+                            __default.ConvertMetaData(response.ResponseMetadata)
+                            ));
+            } catch {
+                return new STL.Result_Failure<DecryptResponse>(new Dafny.Sequence<char>("Exception in KMS.Decypt()".ToCharArray()));
+            }
+        }
+    }
+}
