src/KMS/KMSUtils.dfy
@@ -1,0 +1,56 @@
+include "../SDK/Materials.dfy"
+include "../StandardLibrary/StandardLibrary.dfy"
+include "../StandardLibrary/UInt.dfy"
+
+module {:extern "KMSUtils"} KMSUtils {
+  import Mat = Materials
+  import opened StandardLibrary
+  import opened UInt = StandardLibrary.UInt
+
+  const PROVIDER_ID := "aws-kms"
+
+  datatype DataKeySpec = AES_128 | AES_256
+
+  datatype ResponseMetadata = ResponseMetadata(metadate: map<string, string>, requestID: string)
+
+  type HttpStatusCode = int // FIXME: Restrict this
+
+
+  datatype GenerateDataKeyRequest = GenerateDataKeyRequest(encryptionContext: Mat.EncryptionContext, grantTokens: seq<string>, keyID: string, numberOfBytes: int32)
+
+  datatype GenerateDataKeyResponse = GenerateDataKeyResponse(ciphertextBlob: seq<uint8>, contentLength: int, httpStatusCode: HttpStatusCode, keyID: string, plaintext: seq<uint8>, responseMetadata: ResponseMetadata)
+  {
+    predicate method IsWellFormed() {
+      StringIs8Bit(keyID) && |keyID| < UINT16_LIMIT && |ciphertextBlob| < UINT16_LIMIT
+    }
+  }
+
+
+  datatype EncryptRequest = EncryptRequest(encryptionContext: Mat.EncryptionContext, grantTokens: seq<string>, keyID: string, plaintext: seq<uint8>)
+
+  datatype EncryptResponse = EncryptResponse(ciphertextBlob: seq<uint8>, contentLength: int, httpStatusCode: HttpStatusCode, keyID: string, responseMetadata: ResponseMetadata)
+  {
+    predicate method IsWellFormed() {
+      StringIs8Bit(keyID) && |keyID| < UINT16_LIMIT && |ciphertextBlob| < UINT16_LIMIT
+    }
+  }
+
+  datatype DecryptRequest = DecryptRequest(ciphertextBlob: seq<uint8>, encryptionContext: Mat.EncryptionContext, grantTokens: seq<string>)
+
+  datatype DecryptResponse = DecryptResponse(contentLength: int, httpStatusCode: HttpStatusCode, keyID: string, plaintext: seq<uint8>, responseMetadata: ResponseMetadata)
+
+  // FIXME: mmtj Is it reasonable to call this a function?
+  function method {:extern} GetClient(region: string): (res: KMSClient)
+
+  // https://docs.aws.amazon.com/sdkfornet/v3/apidocs/items/KeyManagementService/TKeyManagementServiceClient.html
+  class KMSClient {
+    method {:extern} GenerateDataKey(request: GenerateDataKeyRequest) returns (res: Result<GenerateDataKeyResponse>)
+      // TODO mmtj: Should this be marked as modifying all of request's fields?
+
+	method {:extern} Encrypt(request: EncryptRequest) returns (res: Result<EncryptResponse>)
+      // TODO mmtj: Should this be marked as modifying all of request's fields?
+
+    method {:extern} Decrypt(request: DecryptRequest) returns (res: Result<DecryptResponse>)
+      // TODO mmtj: Should this be marked as modifying all of request's fields?
+  }
+}
