src/SDK/Keyring/KMSKeyring.dfy
@@ -1,0 +1,205 @@
+include "./Defs.dfy"
+include "../Materials.dfy"
+include "../../StandardLibrary/StandardLibrary.dfy"
+include "../../KMS/KMSUtils.dfy"
+
+module KMSKeyring {
+  import opened StandardLibrary
+  import opened UInt = StandardLibrary.UInt
+  import KeyringDefs
+  import Mat = Materials
+  import KMSUtils
+
+  class KMSKeyring extends KeyringDefs.Keyring {
+
+    const clientSupplier: string -> KMSUtils.KMSClient
+    const keyIDs: seq<string>
+    const generator: Option<string>
+    const grantTokens: seq<string>
+    const isDiscovery: bool
+
+    /*
+    * Does not correctly handle alias strings.
+    * Also it could probably be a function
+    */
+    method RegionFromKMSKeyARN(arn: string) returns (res: Result<string>) {
+      // arn:aws:kms:us-east-1:999999999999:key/01234567-89ab-cdef-fedc-ba9876543210
+      if ':' !in arn {
+        return Failure("Malformed ARN");
+      }
+
+      var start, end := 0, 0;
+      end := StringFind(arn, ':', start);
+      if arn[start..end] != "arn" {
+        return Failure("Malformed ARN");
+      }
+      start := end + 1;
+
+      if ':' !in arn[start..] {
+        return Failure("Malformed ARN");
+      }
+
+      end := StringFind(arn, ':', start);
+      start := end + 1;
+
+      if ':' !in arn[start..] {
+        return Failure("Malformed ARN");
+      }
+
+      end := StringFind(arn, ':', start);
+      if arn[start..end] != "kms" {
+        return Failure("Malformed ARN");
+      }
+      start := end + 1;
+
+      if ':' !in arn[start..] {
+        return Failure("Malformed ARN");
+      }
+
+      end := StringFind(arn, ':', start);
+      return Success(arn[start..end]);
+    }
+
+    predicate Valid() reads this, Repr {
+      Repr == {this} &&
+      |keyIDs| == 0 && generator.None? ==> isDiscovery
+    }
+
+    constructor(clientSupplier: string -> KMSUtils.KMSClient, keyIDs: seq<string>, generator: Option<string>, grantTokens: seq<string>)
+      ensures Valid()
+    {
+      this.clientSupplier := clientSupplier;
+      this.keyIDs         := keyIDs;
+      this.generator      := generator;
+      this.grantTokens    := grantTokens;
+
+      this.isDiscovery    := |keyIDs| == 0 && generator.None?;
+    }
+
+    method GenerateAndSetKey(encMat: Mat.EncryptionMaterials) returns (res: Result<()>)
+      requires Valid()
+      requires encMat.Valid()
+      requires encMat.plaintextDataKey.None?
+      requires generator.Some?
+      requires !isDiscovery
+      modifies encMat`plaintextDataKey, encMat`encryptedDataKeys
+      ensures Valid()
+      ensures res.Success? ==> encMat.Valid() && encMat.plaintextDataKey.Some? && |encMat.encryptedDataKeys| > 0 &&
+                               encMat.encryptedDataKeys[..|encMat.encryptedDataKeys| - 1] == old(encMat.encryptedDataKeys)
+      // TODO: ensure GENERATED_DATA_KEY flag
+    {
+      var generatorRequest := KMSUtils.GenerateDataKeyRequest(encMat.encryptionContext, grantTokens, generator.get, encMat.algorithmSuiteID.KeyLength() as int32);
+      var region :- RegionFromKMSKeyARN(generator.get);
+      var client := clientSupplier(region);
+      var generatorResponse :- client.GenerateDataKey(generatorRequest);
+      if !generatorResponse.IsWellFormed() {
+        return Failure("Invalid response from KMS GenerateDataKey");
+      }
+      var encryptedDataKey := generatorResponse.ciphertextBlob;
+      var keyID := generatorResponse.keyID;
+      var plaintextDataKey := generatorResponse.plaintext;
+
+      if |plaintextDataKey| != encMat.algorithmSuiteID.KeyLength() {
+        return Failure("Invalid response from KMS GenerateDataKey: bad key length");
+      }
+
+      encMat.SetPlaintextDataKey(plaintextDataKey);
+      encMat.AppendEncryptedDataKey(Mat.EncryptedDataKey(KMSUtils.PROVIDER_ID, StringToByteSeq(keyID), encryptedDataKey));
+      return Success(());
+    }
+
+    method OnEncrypt(encMat: Mat.EncryptionMaterials) returns (res: Result<Mat.EncryptionMaterials>)
+      requires Valid()
+      requires encMat.Valid()
+      modifies encMat`plaintextDataKey, encMat`encryptedDataKeys
+      ensures Valid()
+      ensures isDiscovery ==> res.Success? && unchanged(res.value)
+      ensures res.Success? ==> res.value.Valid() && res.value == encMat
+      ensures res.Success? && old(encMat.plaintextDataKey.Some?) ==> res.value.plaintextDataKey == old(encMat.plaintextDataKey)
+      // ensures res.Failure? ==> unchanged(encMat)
+      // TODO: keyring trace GENERATED_DATA_KEY flag assurance
+      // TODO: keyring trace ENCRYPTED_DATA_KEY flag assurance
+    {
+      var encryptCMKs := keyIDs;
+
+      if isDiscovery {
+        return Success(encMat);
+      } else if encMat.plaintextDataKey.None? && generator.None? {
+        return Failure("No plaintext datakey or generator defined");
+      }
+
+      if generator.Some? {
+        if encMat.plaintextDataKey.None? {
+          var _ :- GenerateAndSetKey(encMat);
+        } else {
+          encryptCMKs := encryptCMKs + [generator.get];
+        }
+      }
+
+      ghost var oldPlaintextDataKey := encMat.plaintextDataKey.get;
+      var i := 0;
+      while i < |encryptCMKs|
+        invariant encMat.plaintextDataKey.Some?
+        invariant encMat.plaintextDataKey.get == oldPlaintextDataKey
+        invariant encMat.Valid()
+      {
+        var encryptRequest := KMSUtils.EncryptRequest(encMat.encryptionContext, grantTokens, encryptCMKs[i], encMat.plaintextDataKey.get);
+        var region :- RegionFromKMSKeyARN(encryptCMKs[i]);
+        var client := clientSupplier(region);
+        var encryptResponse :- client.Encrypt(encryptRequest);
+        if encryptResponse.IsWellFormed() {
+          encMat.AppendEncryptedDataKey(Mat.EncryptedDataKey(KMSUtils.PROVIDER_ID, StringToByteSeq(encryptResponse.keyID), encryptResponse.ciphertextBlob));
+        } else {
+          return Failure("Invalid response from KMS Encrypt");
+        }
+        i := i + 1;
+      }
+      return Success(encMat);
+    }
+
+    predicate method DecryptableEDK(edk: Mat.EncryptedDataKey)
+    {
+      edk.providerID == KMSUtils.PROVIDER_ID &&
+      (isDiscovery || ByteSeqToString(edk.providerInfo) in keyIDs)
+    }
+
+    method OnDecrypt(decMat: Mat.DecryptionMaterials, edks: seq<Mat.EncryptedDataKey>) returns (res: Result<Mat.DecryptionMaterials>)
+      requires Valid()
+      requires decMat.Valid()
+      modifies decMat`plaintextDataKey
+      ensures Valid()
+      ensures decMat.Valid()
+      ensures |edks| == 0 ==> res.Success? && unchanged(decMat)
+      ensures old(decMat.plaintextDataKey.Some?) ==> res.Success? && unchanged(decMat)
+      ensures res.Success? ==> res.value == decMat
+      ensures res.Failure? ==> unchanged(decMat)
+      // TODO: keyring trace DECRYPTED_DATA_KEY flag assurance
+      {
+        if |edks| == 0 || decMat.plaintextDataKey.Some? {
+          return Success(decMat);
+        }
+        var decryptableEDKs := Filter(edks, DecryptableEDK);
+        var i := 0;
+        while i < |decryptableEDKs|
+          invariant unchanged(decMat)
+        {
+          var edk := decryptableEDKs[i];
+          var decryptRequest := KMSUtils.DecryptRequest(edk.ciphertext, decMat.encryptionContext, grantTokens);
+          var region :- RegionFromKMSKeyARN(ByteSeqToString(edk.providerInfo));
+          var client := clientSupplier(region);
+          var decryptResponseResult := client.Decrypt(decryptRequest);
+          if decryptResponseResult.Success? {
+            var decryptResponse := decryptResponseResult.value;
+            if decryptResponse.keyID != ByteSeqToString(edk.providerInfo) || |decryptResponse.plaintext| != decMat.algorithmSuiteID.KeyLength() {
+              return Failure("Invalid response from KMS Decrypt");
+            } else {
+              decMat.setPlaintextDataKey(decryptResponse.plaintext);
+              return Success(decMat);
+            }
+          }
+          i := i + 1;
+        }
+        return Success(decMat);
+      }
+  }
+}
